dist/gcc-compatible/EverCrypt_Hash.h
@@ -47,235 +47,46 @@ extern "C" {
 #include "EverCrypt_Error.h"
 #include "EverCrypt_AutoConfig2.h"
 
-typedef Spec_Hash_Definitions_hash_alg EverCrypt_Hash_alg;
-
-C_String_t EverCrypt_Hash_string_of_alg(Spec_Hash_Definitions_hash_alg uu___);
-
-typedef Spec_Hash_Definitions_hash_alg EverCrypt_Hash_broken_alg;
-
-typedef Spec_Hash_Definitions_hash_alg EverCrypt_Hash_alg13;
-
-typedef void *EverCrypt_Hash_e_alg;
-
 typedef struct EverCrypt_Hash_state_s_s EverCrypt_Hash_state_s;
 
-bool
-EverCrypt_Hash_uu___is_MD5_s(
-  Spec_Hash_Definitions_hash_alg uu___,
-  EverCrypt_Hash_state_s projectee
-);
-
-bool
-EverCrypt_Hash_uu___is_SHA1_s(
-  Spec_Hash_Definitions_hash_alg uu___,
-  EverCrypt_Hash_state_s projectee
-);
-
-bool
-EverCrypt_Hash_uu___is_SHA2_224_s(
-  Spec_Hash_Definitions_hash_alg uu___,
-  EverCrypt_Hash_state_s projectee
-);
-
-bool
-EverCrypt_Hash_uu___is_SHA2_256_s(
-  Spec_Hash_Definitions_hash_alg uu___,
-  EverCrypt_Hash_state_s projectee
-);
-
-bool
-EverCrypt_Hash_uu___is_SHA2_384_s(
-  Spec_Hash_Definitions_hash_alg uu___,
-  EverCrypt_Hash_state_s projectee
-);
-
-bool
-EverCrypt_Hash_uu___is_SHA2_512_s(
-  Spec_Hash_Definitions_hash_alg uu___,
-  EverCrypt_Hash_state_s projectee
-);
-
-bool
-EverCrypt_Hash_uu___is_SHA3_256_s(
-  Spec_Hash_Definitions_hash_alg uu___,
-  EverCrypt_Hash_state_s projectee
-);
-
-bool
-EverCrypt_Hash_uu___is_Blake2S_s(
-  Spec_Hash_Definitions_hash_alg uu___,
-  EverCrypt_Hash_state_s projectee
-);
-
-bool
-EverCrypt_Hash_uu___is_Blake2S_128_s(
-  Spec_Hash_Definitions_hash_alg uu___,
-  EverCrypt_Hash_state_s projectee
-);
-
-bool
-EverCrypt_Hash_uu___is_Blake2B_s(
-  Spec_Hash_Definitions_hash_alg uu___,
-  EverCrypt_Hash_state_s projectee
-);
-
-bool
-EverCrypt_Hash_uu___is_Blake2B_256_s(
-  Spec_Hash_Definitions_hash_alg uu___,
-  EverCrypt_Hash_state_s projectee
-);
-
-typedef EverCrypt_Hash_state_s *EverCrypt_Hash_state;
-
-Spec_Hash_Definitions_hash_alg EverCrypt_Hash_alg_of_state(EverCrypt_Hash_state_s *s);
-
-EverCrypt_Hash_state_s *EverCrypt_Hash_create_in(Spec_Hash_Definitions_hash_alg a);
-
-EverCrypt_Hash_state_s *EverCrypt_Hash_create(Spec_Hash_Definitions_hash_alg a);
-
-void EverCrypt_Hash_init(EverCrypt_Hash_state_s *s);
-
-void EverCrypt_Hash_update_multi_256(uint32_t *s, uint8_t *blocks, uint32_t n);
-
-void EverCrypt_Hash_update(EverCrypt_Hash_state_s *s, uint64_t prevlen, uint8_t *block);
-
-void
-EverCrypt_Hash_update_multi(
-  EverCrypt_Hash_state_s *s,
-  uint64_t prevlen,
-  uint8_t *blocks,
-  uint32_t len
-);
-
-void
-EverCrypt_Hash_update_last_256(
-  uint32_t *s,
-  uint64_t input,
-  uint8_t *input_len,
-  uint32_t input_len1
-);
-
-void
-EverCrypt_Hash_update_last(
-  EverCrypt_Hash_state_s *s,
-  uint64_t prev_len,
-  uint8_t *last,
-  uint32_t last_len
-);
-
-void EverCrypt_Hash_finish(EverCrypt_Hash_state_s *s, uint8_t *dst);
-
-void EverCrypt_Hash_free(EverCrypt_Hash_state_s *s);
-
-void EverCrypt_Hash_copy(EverCrypt_Hash_state_s *s_src, EverCrypt_Hash_state_s *s_dst);
-
-void EverCrypt_Hash_hash_256(uint8_t *input, uint32_t input_len, uint8_t *dst);
-
-void EverCrypt_Hash_hash_224(uint8_t *input, uint32_t input_len, uint8_t *dst);
-
-void
-EverCrypt_Hash_hash(
-  Spec_Hash_Definitions_hash_alg a,
-  uint8_t *dst,
-  uint8_t *input,
-  uint32_t len
-);
-
-uint32_t EverCrypt_Hash_Incremental_hash_len(Spec_Hash_Definitions_hash_alg a);
-
-uint32_t EverCrypt_Hash_Incremental_block_len(Spec_Hash_Definitions_hash_alg a);
-
-typedef struct Hacl_Streaming_Functor_state_s___EverCrypt_Hash_state_s_____s
+typedef struct EverCrypt_Hash_Incremental_hash_state_s
 {
   EverCrypt_Hash_state_s *block_state;
   uint8_t *buf;
   uint64_t total_len;
 }
-Hacl_Streaming_Functor_state_s___EverCrypt_Hash_state_s____;
+EverCrypt_Hash_Incremental_hash_state;
 
-Hacl_Streaming_Functor_state_s___EverCrypt_Hash_state_s____
+EverCrypt_Hash_Incremental_hash_state
 *EverCrypt_Hash_Incremental_create_in(Spec_Hash_Definitions_hash_alg a);
 
-void
-EverCrypt_Hash_Incremental_init(Hacl_Streaming_Functor_state_s___EverCrypt_Hash_state_s____ *s);
+void EverCrypt_Hash_Incremental_init(EverCrypt_Hash_Incremental_hash_state *s);
 
 EverCrypt_Error_error_code
 EverCrypt_Hash_Incremental_update(
-  Hacl_Streaming_Functor_state_s___EverCrypt_Hash_state_s____ *s,
+  EverCrypt_Hash_Incremental_hash_state *s,
   uint8_t *data,
   uint32_t len
 );
 
-void
-EverCrypt_Hash_Incremental_finish_md5(
-  Hacl_Streaming_Functor_state_s___EverCrypt_Hash_state_s____ *p,
-  uint8_t *dst
-);
-
-void
-EverCrypt_Hash_Incremental_finish_sha1(
-  Hacl_Streaming_Functor_state_s___EverCrypt_Hash_state_s____ *p,
-  uint8_t *dst
-);
-
-void
-EverCrypt_Hash_Incremental_finish_sha224(
-  Hacl_Streaming_Functor_state_s___EverCrypt_Hash_state_s____ *p,
-  uint8_t *dst
-);
-
-void
-EverCrypt_Hash_Incremental_finish_sha256(
-  Hacl_Streaming_Functor_state_s___EverCrypt_Hash_state_s____ *p,
-  uint8_t *dst
-);
-
-void
-EverCrypt_Hash_Incremental_finish_sha3_256(
-  Hacl_Streaming_Functor_state_s___EverCrypt_Hash_state_s____ *p,
-  uint8_t *dst
-);
-
-void
-EverCrypt_Hash_Incremental_finish_sha384(
-  Hacl_Streaming_Functor_state_s___EverCrypt_Hash_state_s____ *p,
-  uint8_t *dst
-);
-
-void
-EverCrypt_Hash_Incremental_finish_sha512(
-  Hacl_Streaming_Functor_state_s___EverCrypt_Hash_state_s____ *p,
-  uint8_t *dst
-);
-
-void
-EverCrypt_Hash_Incremental_finish_blake2s(
-  Hacl_Streaming_Functor_state_s___EverCrypt_Hash_state_s____ *p,
-  uint8_t *dst
-);
-
-void
-EverCrypt_Hash_Incremental_finish_blake2b(
-  Hacl_Streaming_Functor_state_s___EverCrypt_Hash_state_s____ *p,
-  uint8_t *dst
-);
-
 Spec_Hash_Definitions_hash_alg
-EverCrypt_Hash_Incremental_alg_of_state(
-  Hacl_Streaming_Functor_state_s___EverCrypt_Hash_state_s____ *s
-);
+EverCrypt_Hash_Incremental_alg_of_state(EverCrypt_Hash_Incremental_hash_state *s);
+
+void EverCrypt_Hash_Incremental_finish(EverCrypt_Hash_Incremental_hash_state *s, uint8_t *dst);
+
+void EverCrypt_Hash_Incremental_free(EverCrypt_Hash_Incremental_hash_state *s);
+
+void EverCrypt_Hash_Incremental_hash_256(uint8_t *input, uint32_t input_len, uint8_t *dst);
+
+void EverCrypt_Hash_Incremental_hash_224(uint8_t *input, uint32_t input_len, uint8_t *dst);
 
 void
-EverCrypt_Hash_Incremental_finish(
-  Hacl_Streaming_Functor_state_s___EverCrypt_Hash_state_s____ *s,
-  uint8_t *dst
+EverCrypt_Hash_Incremental_hash(
+  Spec_Hash_Definitions_hash_alg a,
+  uint8_t *dst,
+  uint8_t *input,
+  uint32_t len
 );
-
-void
-EverCrypt_Hash_Incremental_free(Hacl_Streaming_Functor_state_s___EverCrypt_Hash_state_s____ *s);
-
-typedef Hacl_Streaming_Functor_state_s___EverCrypt_Hash_state_s____
-*EverCrypt_Hash_Incremental_state;
 
 #if defined(__cplusplus)
 }
