dist/gcc-compatible/Hacl_Hash_MD5.c
@@ -56,7 +56,7 @@ void Hacl_Hash_Core_MD5_legacy_init(uint32_t *s)
   KRML_MAYBE_FOR4(i, (uint32_t)0U, (uint32_t)4U, (uint32_t)1U, s[i] = _h0[i];);
 }
 
-void Hacl_Hash_Core_MD5_legacy_update(uint32_t *abcd, uint8_t *x)
+static void legacy_update(uint32_t *abcd, uint8_t *x)
 {
   uint32_t aa = abcd[0U];
   uint32_t bb = abcd[1U];
@@ -1136,7 +1136,7 @@ void Hacl_Hash_MD5_legacy_update_multi(uint32_t *s, uint8_t *blocks, uint32_t n_
   {
     uint32_t sz = (uint32_t)64U;
     uint8_t *block = blocks + sz * i;
-    Hacl_Hash_Core_MD5_legacy_update(s, block);
+    legacy_update(s, block);
   }
 }
 
