dist/gcc-compatible/internal/Hacl_Hash_Blake2b_256.h
@@ -41,13 +41,6 @@ extern "C" {
 FStar_UInt128_uint128
 Hacl_Hash_Blake2b_256_init_blake2b_256(Lib_IntVector_Intrinsics_vec256 *s);
 
-FStar_UInt128_uint128
-Hacl_Hash_Blake2b_256_update_blake2b_256(
-  Lib_IntVector_Intrinsics_vec256 *s,
-  FStar_UInt128_uint128 totlen,
-  uint8_t *block
-);
-
 void
 Hacl_Hash_Blake2b_256_finish_blake2b_256(
   Lib_IntVector_Intrinsics_vec256 *s,
