providers/evercrypt/fst/EverCrypt.Hash.Incremental.fst
@@ -27,6 +27,9 @@ open Spec.Hash.Incremental.Lemmas
 
 #set-options "--z3rlimit 200 --max_fuel 0 --max_ifuel 0"
 
+// Definitions for instantiating the streaming functor
+// ---------------------------------------------------
+
 inline_for_extraction noextract
 let agile_state: stateful hash_alg =
   Stateful
@@ -49,6 +52,7 @@ let agile_state: stateful hash_alg =
     (fun i -> EverCrypt.Hash.free #i)
     (fun i -> EverCrypt.Hash.copy #i)
 
+
 #push-options "--ifuel 1"
 inline_for_extraction noextract
 let mk_words_state (#a : hash_alg) (s : words_state' a)
@@ -60,7 +64,10 @@ let mk_words_state (#a : hash_alg) (s : words_state' a)
 #pop-options
 
 (* Adding some non-inlined definitions to factorize code *)
+private
 let hash_len a = Hacl.Hash.Definitions.hash_len a
+
+private
 let block_len a = Hacl.Hash.Definitions.block_len a
 
 val hash_is_hash_incremental (a: hash_alg)
@@ -143,6 +150,13 @@ let evercrypt_hash : block hash_alg =
     (fun i _ -> EverCrypt.Hash.finish #i)
 #pop-options
 
+// Monomorphization hint. The index is eventually ghost so SHA2_256 is just a dummy here.
+let hash_state =
+  F.state_s evercrypt_hash SHA2_256 ((agile_state).s SHA2_256) (G.erased unit)
+
+// Public API (streaming)
+// ----------------------
+
 let create_in a = F.create_in evercrypt_hash a (EverCrypt.Hash.state a) (G.erased unit) ()
 
 let init (a: G.erased hash_alg) = F.init evercrypt_hash a (EverCrypt.Hash.state a) (G.erased unit) ()
@@ -172,14 +186,23 @@ let finish_st a = F.finish_st evercrypt_hash a (EverCrypt.Hash.state a) (G.erase
 
 /// The wrapper pattern, to ensure that the stack-allocated state is properly
 /// monomorphized.
+private
 let finish_md5: finish_st MD5 = F.mk_finish evercrypt_hash MD5 (EverCrypt.Hash.state MD5) (G.erased unit)
+private
 let finish_sha1: finish_st SHA1 = F.mk_finish evercrypt_hash SHA1 (EverCrypt.Hash.state SHA1) (G.erased unit)
+private
 let finish_sha224: finish_st SHA2_224 = F.mk_finish evercrypt_hash SHA2_224 (EverCrypt.Hash.state SHA2_224) (G.erased unit)
+private
 let finish_sha256: finish_st SHA2_256 = F.mk_finish evercrypt_hash SHA2_256 (EverCrypt.Hash.state SHA2_256) (G.erased unit)
+private
 let finish_sha3_256: finish_st SHA3_256 = F.mk_finish evercrypt_hash SHA3_256 (EverCrypt.Hash.state SHA3_256) (G.erased unit)
+private
 let finish_sha384: finish_st SHA2_384 = F.mk_finish evercrypt_hash SHA2_384 (EverCrypt.Hash.state SHA2_384) (G.erased unit)
+private
 let finish_sha512: finish_st SHA2_512 = F.mk_finish evercrypt_hash SHA2_512 (EverCrypt.Hash.state SHA2_512) (G.erased unit)
+private
 let finish_blake2s: finish_st Blake2S = F.mk_finish evercrypt_hash Blake2S (EverCrypt.Hash.state Blake2S) (G.erased unit)
+private
 let finish_blake2b: finish_st Blake2B = F.mk_finish evercrypt_hash Blake2B (EverCrypt.Hash.state Blake2B) (G.erased unit)
 
 let alg_of_state (a: G.erased hash_alg) = F.index_of_state evercrypt_hash a (EverCrypt.Hash.state a) (G.erased unit)
@@ -200,9 +223,76 @@ let finish a s dst =
 
 let free (i: G.erased hash_alg) = F.free evercrypt_hash i (EverCrypt.Hash.state i) (G.erased unit)
 
-/// Finally, a few helpers predicates to make things easier for clients...
+// Public API (one-shot, multiplexing)
+// -----------------------------------
 
+val hash_256: Hacl.Hash.Definitions.hash_st SHA2_256
+
+val hash_224: Hacl.Hash.Definitions.hash_st SHA2_224
+
+// A full one-shot hash that relies on vale at each multiplexing point
+let hash_256 input input_len dst =
+  let open EverCrypt.Hash in
+  Hacl.Hash.MD.mk_hash SHA2_256 Hacl.Hash.SHA2.alloca_256 update_multi_256
+    update_last_256 Hacl.Hash.SHA2.finish_256 input input_len dst
+
+let hash_224 input input_len dst =
+  let open EverCrypt.Hash in
+  Hacl.Hash.MD.mk_hash SHA2_224 Hacl.Hash.SHA2.alloca_224 update_multi_224
+    update_last_224 Hacl.Hash.SHA2.finish_224 input input_len dst
+
+// Public API (one-shot, agile and multiplexing)
+// ---------------------------------------------
+
+(** @type: true
+*)
+val hash:
+  a:Spec.Agile.Hash.hash_alg ->
+  dst:B.buffer Lib.IntTypes.uint8 {B.length dst = hash_length a} ->
+  input:B.buffer Lib.IntTypes.uint8 ->
+  len:FStar.UInt32.t {B.length input = FStar.UInt32.v len /\ FStar.UInt32.v len `less_than_max_input_length` a} ->
+  Stack unit
+  (requires fun h0 ->
+    B.live h0 dst /\
+    B.live h0 input /\
+    B.(loc_disjoint (loc_buffer input) (loc_buffer dst)))
+  (ensures fun h0 _ h1 ->
+    B.(modifies (loc_buffer dst) h0 h1) /\
+    B.as_seq h1 dst == Spec.Agile.Hash.hash a (B.as_seq h0 input))
+
+// NOTE: this function goes through all the Hacl.Hash.* wrappers which export
+// the correct agile low-level type, and thus does not need to be aware of the
+// implementation of Spec.Agile.Hash (no friend-ing).
+let hash a dst input len =
+  let _ = allow_inversion Spec.Agile.Hash.hash_alg in
+  match a with
+  | MD5 -> Hacl.Hash.MD5.legacy_hash input len dst
+  | SHA1 -> Hacl.Hash.SHA1.legacy_hash input len dst
+  | SHA2_224 -> hash_224 input len dst
+  | SHA2_256 -> hash_256 input len dst
+  | SHA2_384 -> Hacl.Hash.SHA2.hash_384 input len dst
+  | SHA2_512 -> Hacl.Hash.SHA2.hash_512 input len dst
+  | SHA3_256 -> Hacl.Hash.SHA3.hash_256 input len dst
+  | Blake2S ->
+      let vec128 = EverCrypt.AutoConfig2.has_vec128 () in
+      if EverCrypt.TargetConfig.hacl_can_compile_vec128 && vec128 then
+        Hacl.Hash.Blake2s_128.hash_blake2s_128 input len dst
+      else
+        Hacl.Hash.Blake2.hash_blake2s_32 input len dst
+  | Blake2B ->
+      let vec256 = EverCrypt.AutoConfig2.has_vec256 () in
+      if EverCrypt.TargetConfig.hacl_can_compile_vec256 && vec256 then
+        Hacl.Hash.Blake2b_256.hash_blake2b_256 input len dst
+      else
+        Hacl.Hash.Blake2.hash_blake2b_32 input len dst
+
+// Public API (verified clients)
+// -----------------------------
+
+/// Finally, a few helpers predicates to make things easier for clients...
+inline_for_extraction noextract
 let state (a: hash_alg) = F.state evercrypt_hash a (EverCrypt.Hash.state a) (G.erased unit)
 
+inline_for_extraction noextract
 let hashed #a (h: HS.mem) (s: state a) =
   F.seen evercrypt_hash a h s
